Suppose we have a probability density function (pdf) defined as:
\begin{align*}
    f(x,y) = \left.
    \begin{cases}
    C(x^2 + 2y), &\text{$0 < x < 1$ and $0 < y < 1$,} \\
    0,    &\text{otherwise.}
   \end{cases}
   \right.
\end{align*}

 \begin{enumerate}
 \item   Find the value of $C$. [2pts]
 \item  Find the marginal distribution of $X$ and $Y$. [4pts]
 \item  Find the joint cumulative density function (cdf) of $X$ and $Y$. [4pts]

  \end{enumerate}

\begin{solution} \ \\
a) 

$\int_{0}^{1}\int_{0}^{1} C(x^2 + 2y) dy dx\\
= \int_{0}^{1}\int_{0}^{1} Cx^2 + 2Cy dy dx\\
= \int_{0}^{1} (Cx^2y + Cy^2)\rvert_0^1 dx\\
= \int_{0}^{1} Cx^2(1) + C(1)^2 - Cx^2(0) - C(0)^2 dx\\
= \int_{0}^{1} Cx^2 + C dx\\
= \frac{1}{3}Cx^3 + Cx \rvert_0^1\\
= \frac{1}{3}C + C\\$
Since f(x, y) is a pdf, we know its integral is 1. Therefore, we need $\frac{1}{3}C + C = 1$:\\
$\frac{1}{3}C + C = 1\\
\implies \frac{4}{3}C = 1\\
\implies C = \frac{3}{4}\\$

$\therefore$ We get $C = \frac{3}{4}$.\\

b) 

$f_X(x) = \int_{0}^{1} \frac{3}{4}(x^2 + 2y) dy\\
= \frac{3}{4}\int_{0}^{1} (x^2 + 2y) dy\\
= \frac{3}{4} (x^2y + y^2)\rvert_0^1\\
= \frac{3}{4} (x^2 + 1)\\
= \frac{3}{4}x^2 + \frac{3}{4}\\
= \left.
\begin{cases}
\frac{3}{4}x^2 + \frac{3}{4}, &\text{$0 < x < 1$,} \\
0,    &\text{otherwise.}
\end{cases}
\right.$\\

$f_Y(y) = \int_{0}^{1} \frac{3}{4}(x^2 + 2y) dx\\
= \frac{3}{4}\int_{0}^{1} (x^2 + 2y) dx\\
= \frac{3}{4} (\frac{1}{3}x^3 + 2yx)\rvert_0^1\\
= \frac{3}{4} (\frac{1}{3} + 2y)\\
= \frac{1}{4} + \frac{3}{2}y\\
= \left.
\begin{cases}
\frac{1}{4} + \frac{3}{2}y, &\text{$0 < y < 1$,} \\
0,    &\text{otherwise.}
\end{cases}
\right.$\\

c) 

We know when $x < 0$ and $y < 0$, f(x, y) = 0, so $F_{XY} = 0$.

We also know that when $x \geq 1$ and $y \geq 1$, $F_{XY} = 1$. 

For $0 \leq x \leq 1$ and $0 \leq y \leq 1$, we need to calculate the following:

$F_{XY}(x, y) = \int_{0}^{y}\int_{0}^{x} \frac{3}{4}(x^2 + 2y) dx dy\\
= \frac{3}{4}\int_{0}^{y}\int_{0}^{x}(x^2 + 2y) dx dy\\
= \frac{3}{4}\int_{0}^{y}(\frac{1}{3}x^3 + 2xy)\rvert_0^x dy\\
= \frac{3}{4}\int_{0}^{y}(\frac{1}{3}x^3 + 2xy) dy\\
= \frac{3}{4}(\frac{1}{3}x^3y + xy^2)\rvert_0^y\\
= \frac{1}{4}x^3y + \frac{3}{4}xy^2$

Now, when $0 \leq x \leq 1$ and $y \geq 1$, we get $F_{XY}(x, y) = F_{XY}(x, 1) = \frac{1}{4}x^3 + \frac{3}{4}x$.

Additionally, when $x \geq 1$ and $0 \leq y \leq 1$, we get $F_{XY}(x, y) = F_{XY}(1, y) = \frac{1}{4}y + \frac{3}{4}y^2$.

So, the joint cdf is as follows:\\

\begin{align*}
	F_{XY}(x,y) = \left.
	\begin{cases}
		0, &\text{$x < 0$ or $y < 0$,} \\
		\frac{1}{4}x^3y + \frac{3}{4}xy^2, &\text{$0 \leq x \leq 1$ and $0 \leq y \leq 1$,} \\
		\frac{1}{4}y + \frac{3}{4}y^2, &\text{$x \geq 1$ and $0 \leq y \leq 1$,} \\
		\frac{1}{4}x^3 + \frac{3}{4}x, &\text{$0 \leq x \leq 1$ and $y \geq 1$,} \\
		1, &\text{$x \geq 1$ and $x \geq 1$,} \\
	\end{cases}
	\right.
\end{align*}
\end{solution}